src/PlutusIR/Semantics/SemanticEquivalence/LogicalRelation/Tymapping.v
@@ -13,13 +13,13 @@ Local Open Scope string_scope.
     and [T2] are, respectively, the ''left'' and ''right'' syntactic substitutions
     for the type variable [a].
 *)
-Definition tymapping := list (tyname * ((nat -> Term -> Term -> Prop) * Ty * Ty)).
+Definition tymapping := list (string * ((nat -> Term -> Term -> Prop) * Ty * Ty)).
 
 
 (* TODO: Rewrite using lookup *)
 
 (** Semantic substitution for the type variable [a] *)
-Fixpoint sem (rho : tymapping) (a : tyname) : option (nat -> Term -> Term -> Prop) :=
+Fixpoint sem (rho : tymapping) (a : string) : option (nat -> Term -> Term -> Prop) :=
   match rho with
   | nil => None
   | (a', (Chi, _ , _)) :: rho' =>
@@ -27,7 +27,7 @@ Fixpoint sem (rho : tymapping) (a : tyname) : option (nat -> Term -> Term -> Pro
   end.
 
 (** (Left) syntactic substitution for the type variable [a] *)
-Fixpoint syn1 (rho : tymapping) (a : tyname) : option Ty :=
+Fixpoint syn1 (rho : tymapping) (a : string) : option Ty :=
   match rho with
   | nil => None
   | (a', (_, T1, _)) :: rho' =>
@@ -35,7 +35,7 @@ Fixpoint syn1 (rho : tymapping) (a : tyname) : option Ty :=
   end.
 
 (** (Right) syntactic substitution for the type variable [a] *)
-Fixpoint syn2 (rho : tymapping) (a : tyname) : option Ty :=
+Fixpoint syn2 (rho : tymapping) (a : string) : option Ty :=
   match rho with
   | nil => None
   | (a', (_, _, T2)) :: rho' =>
@@ -43,7 +43,7 @@ Fixpoint syn2 (rho : tymapping) (a : tyname) : option Ty :=
   end.
 
 (** (Left) syntactic substitutions in [rho] *)
-Fixpoint msyn1 (rho : tymapping) : list (tyname * Ty) :=
+Fixpoint msyn1 (rho : tymapping) : list (string * Ty) :=
   match rho with
   | nil => nil
   | (a', (_, T1, _)) :: rho' =>
@@ -51,7 +51,7 @@ Fixpoint msyn1 (rho : tymapping) : list (tyname * Ty) :=
   end.
 
 (** (Right) syntactic substitutions in [rho] *)
-Fixpoint msyn2 (rho : tymapping) : list (tyname * Ty) :=
+Fixpoint msyn2 (rho : tymapping) : list (string * Ty) :=
   match rho with
   | nil => nil
   | (a', (_, _, T2)) :: rho' =>
